begun formatting

Adaptive_State_Counting/ATC/ATC.thy
@@ -18,9 +18,12 @@ a leaf.
 
 datatype ('in, 'out) ATC = Leaf | Node 'in "'out \<Rightarrow> ('in, 'out) ATC"
 
-inductive atc_reaction :: "('in, 'out, 'state) FSM \<Rightarrow> 'state \<Rightarrow> ('in, 'out) ATC \<Rightarrow> ('in \<times> 'out) list \<Rightarrow> bool" where
+inductive atc_reaction :: 
+  "('in, 'out, 'state) FSM \<Rightarrow> 'state \<Rightarrow> ('in, 'out) ATC \<Rightarrow> ('in \<times> 'out) list \<Rightarrow> bool" where
   leaf[intro!]: "atc_reaction M q1 Leaf []" |
-  node[intro!]: "q2 \<in> succ M (x,y) q1 \<Longrightarrow> atc_reaction M q2 (f y) io \<Longrightarrow> atc_reaction M q1 (Node x f) ((x,y)#io)"
+  node[intro!]: "q2 \<in> succ M (x,y) q1 
+                  \<Longrightarrow> atc_reaction M q2 (f y) io 
+                  \<Longrightarrow> atc_reaction M q1 (Node x f) ((x,y)#io)"
 
 inductive_cases leaf_elim[elim!] : "atc_reaction M q1 Leaf []"
 inductive_cases node_elim[elim!] : "atc_reaction M q1 (Node x f) ((x,y)#io)"
@@ -51,9 +54,12 @@ lemma atc_reaction_nonempty[elim] :
   obtains q2 f 
   where "t = Node x f" "q2 \<in> succ M (x,y) q1"  "atc_reaction M q2 (f y) io"
 proof -
-  obtain x2 f where "t = Node x2 f"  using assms by (metis ATC.exhaust atc_reaction_nonempty_no_leaf) 
-  moreover have "x = x2" using assms calculation atc_reaction.cases by fastforce 
-  ultimately show ?thesis using assms using that by blast 
+  obtain x2 f where "t = Node x2 f"  
+    using assms by (metis ATC.exhaust atc_reaction_nonempty_no_leaf) 
+  moreover have "x = x2" 
+    using assms calculation atc_reaction.cases by fastforce 
+  ultimately show ?thesis 
+    using assms using that by blast 
 qed
 
 lemma atc_reaction_path_ex : 
@@ -64,11 +70,16 @@ using assms proof (induction io arbitrary: q1 t rule: list.induct)
   then show ?case by (simp add: FSM.nil) 
 next
   case (Cons io_hd io_tl)
-  then obtain x y where io_hd_def : "io_hd = (x,y)" by (meson surj_pair)
-  then obtain f where f_def : "t = (Node x f)" using Cons atc_reaction_nonempty by metis
-  then obtain q2 where q2_def : "q2 \<in> succ M (x,y) q1" "atc_reaction M q2 (f y) io_tl" using Cons io_hd_def atc_reaction_nonempty by auto
-  then obtain tr_tl where tr_tl_def :  "path M (io_tl || tr_tl) q2" "length io_tl = length tr_tl" using Cons.IH[of q2 "f y"] by blast
-  then have "path M (io_hd # io_tl || q2 # tr_tl) q1" using Cons q2_def by (simp add: FSM.path.intros(2) io_hd_def)
+  then obtain x y where io_hd_def : "io_hd = (x,y)" 
+    by (meson surj_pair)
+  then obtain f where f_def : "t = (Node x f)" 
+    using Cons atc_reaction_nonempty by metis
+  then obtain q2 where q2_def : "q2 \<in> succ M (x,y) q1" "atc_reaction M q2 (f y) io_tl" 
+    using Cons io_hd_def atc_reaction_nonempty by auto
+  then obtain tr_tl where tr_tl_def :  "path M (io_tl || tr_tl) q2" "length io_tl = length tr_tl" 
+    using Cons.IH[of q2 "f y"] by blast
+  then have "path M (io_hd # io_tl || q2 # tr_tl) q1" 
+    using Cons q2_def by (simp add: FSM.path.intros(2) io_hd_def)
   then show ?case using tr_tl_def by fastforce   
 qed
 
@@ -133,7 +144,7 @@ lemma applicable_subtest :
   assumes "applicable M (Node x f)"
 shows "applicable M (f y)"
 using assms inputs_atc.simps
-by (simp add: Sup_le_iff)
+  by (simp add: Sup_le_iff)
 
 
 
@@ -146,7 +157,8 @@ Function IO collects all ATC-reactions of some FSM to some ATC.
 fun IO :: "('in, 'out, 'state) FSM \<Rightarrow> 'state \<Rightarrow> ('in, 'out) ATC \<Rightarrow> ('in \<times> 'out) list set" where
   "IO M q t = { tr . atc_reaction M q t tr }"
 
-fun IO_set :: "('in, 'out, 'state) FSM \<Rightarrow> 'state \<Rightarrow> ('in, 'out) ATC set \<Rightarrow> ('in \<times> 'out) list set" where
+fun IO_set :: "('in, 'out, 'state) FSM \<Rightarrow> 'state \<Rightarrow> ('in, 'out) ATC set \<Rightarrow> ('in \<times> 'out) list set" 
+  where
   "IO_set M q \<Omega> = \<Union> {IO M q t | t . t \<in> \<Omega>}"
 
 lemma IO_language : "IO M q t \<subseteq> language_state M q"
@@ -157,8 +169,10 @@ proof
   show "IO M q Leaf \<subseteq> {[]}" 
   proof (rule ccontr)
     assume assm : "\<not> IO M q Leaf \<subseteq> {[]}"
-    then obtain io_hd io_tl where elem_ex : "Cons io_hd io_tl \<in> IO M q Leaf" by (metis (no_types, hide_lams) insertI1 neq_Nil_conv subset_eq) 
-    then show "False" using atc_reaction_nonempty_no_leaf assm by (metis IO.simps mem_Collect_eq)
+    then obtain io_hd io_tl where elem_ex : "Cons io_hd io_tl \<in> IO M q Leaf" 
+      by (metis (no_types, hide_lams) insertI1 neq_Nil_conv subset_eq) 
+    then show "False" 
+      using atc_reaction_nonempty_no_leaf assm by (metis IO.simps mem_Collect_eq)
   qed  
 next
   show "{[]} \<subseteq> IO M q Leaf" by auto 
@@ -176,12 +190,16 @@ using assms proof (induction t arbitrary: q1)
 next
   case (Node x f)
   then have "x \<in> inputs M" by auto
-  then obtain y q2  where x_appl : "q2 \<in> succ M (x, y) q1" using Node unfolding completely_specified.simps by blast
-  then have "applicable M (f y)" using applicable_subtest Node by metis
+  then obtain y q2  where x_appl : "q2 \<in> succ M (x, y) q1" 
+    using Node unfolding completely_specified.simps by blast
+  then have "applicable M (f y)" 
+    using applicable_subtest Node by metis
   moreover have "q2 \<in> nodes M" 
     using Node(4) \<open>q2 \<in> succ M (x, y) q1\<close> FSM.nodes.intros(2)[of q1 M "((x,y),q2)"] by auto
-  ultimately have "IO M q2 (f y) \<noteq> {}" using Node by auto
-  then show ?case unfolding IO.simps using x_appl by blast  
+  ultimately have "IO M q2 (f y) \<noteq> {}" 
+    using Node by auto
+  then show ?case unfolding IO.simps 
+    using x_appl by blast  
 qed
 
 
@@ -215,10 +233,14 @@ lemma r_dist_dist :
 shows   "q1 \<noteq> q2"
 proof (rule ccontr)
   assume "\<not>(q1 \<noteq> q2)" 
-  then have "q1 = q2" by simp
-  then have "IO M q1 t = {}" using assms by simp
-  moreover have "IO M q1 t \<noteq> {}" using assms IO_applicable_nonempty by auto
-  ultimately show "False" by simp
+  then have "q1 = q2" 
+    by simp
+  then have "IO M q1 t = {}" 
+    using assms by simp
+  moreover have "IO M q1 t \<noteq> {}" 
+    using assms IO_applicable_nonempty by auto
+  ultimately show "False" 
+    by simp
 qed
 
 lemma r_dist_set_dist :
@@ -249,15 +271,18 @@ ATCs on every state reached in some FSM using a given set of IO-sequences.
 \<close>
 
 
-fun B :: "('in, 'out, 'state) FSM \<Rightarrow> ('in * 'out) list \<Rightarrow> ('in, 'out) ATC set \<Rightarrow> ('in * 'out) list set" where
-"B M io \<Omega> = \<Union> (image (\<lambda> s . IO_set M s \<Omega>) (io_targets M (initial M) io))"
+fun B :: "('in, 'out, 'state) FSM \<Rightarrow> ('in * 'out) list \<Rightarrow> ('in, 'out) ATC set 
+          \<Rightarrow> ('in * 'out) list set" where
+  "B M io \<Omega> = \<Union> (image (\<lambda> s . IO_set M s \<Omega>) (io_targets M (initial M) io))"
 
 
-fun D :: "('in, 'out, 'state) FSM \<Rightarrow> ('in, 'out) ATC set \<Rightarrow> 'in list set \<Rightarrow> ('in * 'out) list set set" where
+fun D :: "('in, 'out, 'state) FSM \<Rightarrow> ('in, 'out) ATC set \<Rightarrow> 'in list set 
+          \<Rightarrow> ('in * 'out) list set set" where
   "D M \<Omega> ISeqs = image (\<lambda> io . B M io \<Omega>) (LS\<^sub>i\<^sub>n M (initial M) ISeqs)"
 
-fun append_io_B :: "('in, 'out, 'state) FSM \<Rightarrow> ('in * 'out) list \<Rightarrow> ('in, 'out) ATC set \<Rightarrow> ('in * 'out) list set" where
-"append_io_B M io \<Omega> = { io@res | res . res \<in> B M io \<Omega> }"
+fun append_io_B :: "('in, 'out, 'state) FSM \<Rightarrow> ('in * 'out) list \<Rightarrow> ('in, 'out) ATC set 
+                    \<Rightarrow> ('in * 'out) list set" where
+  "append_io_B M io \<Omega> = { io@res | res . res \<in> B M io \<Omega> }"
 
 
 
@@ -284,14 +309,23 @@ proof -
   have "D M \<Omega> ISeqs \<subseteq> image (\<lambda> s . IO_set M s \<Omega>) (nodes M)"
   proof 
     fix RS assume RS_def : "RS \<in> D M \<Omega> ISeqs"
-    then obtain xs ys where RS_tr : "RS = B M (xs || ys) \<Omega>" "(xs \<in> ISeqs \<and> length xs = length ys \<and> (xs || ys) \<in> language_state M (initial M))"by auto
-    then obtain qx where qx_def : "io_targets M (initial M) (xs || ys) = { qx }" by (meson io_targets_observable_singleton_ex ob)  
-    then have "RS = IO_set M qx \<Omega>" using RS_tr by auto
-    moreover have "qx \<in> nodes M" by (metis FSM.nodes.initial io_targets_nodes qx_def singletonI) 
-    ultimately show "RS \<in> image (\<lambda> s . IO_set M s \<Omega>) (nodes M)" by auto
+    then obtain xs ys where RS_tr : "RS = B M (xs || ys) \<Omega>" 
+                                    "(xs \<in> ISeqs \<and> length xs = length ys 
+                                        \<and> (xs || ys) \<in> language_state M (initial M))" 
+      by auto
+    then obtain qx where qx_def : "io_targets M (initial M) (xs || ys) = { qx }" 
+      by (meson io_targets_observable_singleton_ex ob)  
+    then have "RS = IO_set M qx \<Omega>" 
+      using RS_tr by auto
+    moreover have "qx \<in> nodes M" 
+      by (metis FSM.nodes.initial io_targets_nodes qx_def singletonI) 
+    ultimately show "RS \<in> image (\<lambda> s . IO_set M s \<Omega>) (nodes M)" 
+      by auto
   qed
-  moreover have "finite (nodes M)" using assms by auto
-  ultimately show "finite (D M \<Omega> ISeqs)" "card (D M \<Omega> ISeqs) \<le> card (nodes M)" by (meson  finite_imageI infinite_super surj_card_le)+
+  moreover have "finite (nodes M)" 
+    using assms by auto
+  ultimately show "finite (D M \<Omega> ISeqs)" "card (D M \<Omega> ISeqs) \<le> card (nodes M)" 
+    by (meson  finite_imageI infinite_super surj_card_le)+
 qed
 
 
@@ -306,7 +340,8 @@ proof
   then have "res \<in> LS M q" 
     using IO_set_in_language[of M q \<Omega>] by blast
 
-  obtain pIO where "path M (io || pIO) (initial M)" "length pIO = length io" "target (io || pIO) (initial M) = q"
+  obtain pIO where "path M (io || pIO) (initial M)" 
+                   "length pIO = length io" "target (io || pIO) (initial M) = q"
     using \<open>q \<in> io_targets M (initial M) io\<close> by auto
   moreover obtain pRes where "path M (res || pRes) q" "length pRes = length res" 
     using \<open>res \<in> LS M q\<close> by auto
@@ -325,17 +360,26 @@ lemma append_io_B_nonempty :
   and     "\<Omega> \<noteq> {}"
 shows "append_io_B M io \<Omega> \<noteq> {}"
 proof -
-  obtain t where "t \<in> \<Omega>" using assms(4) by blast
-  then have "applicable M t" using assms(1) by simp
-  moreover obtain tr where "path M (io || tr) (initial M) \<and> length tr = length io" using assms(3) by auto
+  obtain t where "t \<in> \<Omega>" 
+    using assms(4) by blast
+  then have "applicable M t" 
+    using assms(1) by simp
+  moreover obtain tr where "path M (io || tr) (initial M) \<and> length tr = length io" 
+    using assms(3) by auto
   moreover have "target (io || tr) (initial M) \<in> nodes M"
     using calculation(2) by blast
-  ultimately have "IO M (target (io || tr) (initial M)) t \<noteq> {}" using assms(2) IO_applicable_nonempty by simp
-  then obtain io' where "io' \<in> IO M (target (io || tr) (initial M)) t" by blast
-  then have "io' \<in> IO_set M (target (io || tr) (initial M)) \<Omega>" using \<open>t \<in> \<Omega>\<close> unfolding IO_set.simps by blast
-  moreover have "(target (io || tr) (initial M)) \<in> io_targets M (initial M) io" using \<open>path M (io || tr) (initial M) \<and> length tr = length io\<close> by auto 
-  ultimately have "io' \<in> B M io \<Omega>" unfolding B.simps by blast
-  then have "io@io' \<in> append_io_B M io \<Omega>" unfolding append_io_B.simps by blast
+  ultimately have "IO M (target (io || tr) (initial M)) t \<noteq> {}" 
+    using assms(2) IO_applicable_nonempty by simp
+  then obtain io' where "io' \<in> IO M (target (io || tr) (initial M)) t" 
+    by blast
+  then have "io' \<in> IO_set M (target (io || tr) (initial M)) \<Omega>" 
+    using \<open>t \<in> \<Omega>\<close> unfolding IO_set.simps by blast
+  moreover have "(target (io || tr) (initial M)) \<in> io_targets M (initial M) io" 
+    using \<open>path M (io || tr) (initial M) \<and> length tr = length io\<close> by auto 
+  ultimately have "io' \<in> B M io \<Omega>" 
+    unfolding B.simps by blast
+  then have "io@io' \<in> append_io_B M io \<Omega>" 
+    unfolding append_io_B.simps by blast
   then show ?thesis by blast
 qed
   
@@ -344,10 +388,14 @@ lemma append_io_B_prefix_in_language :
   assumes "append_io_B M io \<Omega> \<noteq> {}"
   shows "io \<in> L M"
 proof -
-  obtain res where "io @ res \<in> append_io_B M io \<Omega> \<and> res \<in> B M io \<Omega>" using assms by auto 
-  then have "io_targets M (initial M) io \<noteq> {}" by auto
-  then obtain q where "q \<in> io_targets M (initial M) io" by blast
-  then obtain tr where "target (io || tr) (initial M) = q \<and> path M (io || tr) (initial M) \<and> length tr = length io" by auto 
+  obtain res where "io @ res \<in> append_io_B M io \<Omega> \<and> res \<in> B M io \<Omega>" 
+    using assms by auto 
+  then have "io_targets M (initial M) io \<noteq> {}" 
+    by auto
+  then obtain q where "q \<in> io_targets M (initial M) io" 
+    by blast
+  then obtain tr where "target (io || tr) (initial M) = q \<and> path M (io || tr) (initial M) 
+                          \<and> length tr = length io" by auto 
   then show ?thesis by auto
 qed
 
@@ -375,8 +423,9 @@ ATC-reaction to it of the former state is also an ATC-reaction of the latter sta
 \<close>
 
 
-fun atc_reduction :: "('in, 'out, 'state) FSM \<Rightarrow> 'state \<Rightarrow> ('in, 'out, 'state) FSM \<Rightarrow> 'state \<Rightarrow> ('in, 'out) ATC set \<Rightarrow> bool" where
-"atc_reduction M2 s2 M1 s1 \<Omega> = (\<forall> t \<in> \<Omega> . IO M2 s2 t \<subseteq> IO M1 s1 t)"
+fun atc_reduction :: "('in, 'out, 'state) FSM \<Rightarrow> 'state \<Rightarrow> ('in, 'out, 'state) FSM \<Rightarrow> 'state 
+                      \<Rightarrow> ('in, 'out) ATC set \<Rightarrow> bool" where
+  "atc_reduction M2 s2 M1 s1 \<Omega> = (\<forall> t \<in> \<Omega> . IO M2 s2 t \<subseteq> IO M1 s1 t)"
 
 
 
@@ -392,16 +441,25 @@ lemma atc_rdist_dist[intro] :
   and             "t1 \<in> nodes M2"
 shows "r_dist_set M2 \<Omega> t1 t2"
 proof -
-  obtain td where td_def : "td \<in> \<Omega> \<and> r_dist M1 td s1 s2" using rdist by auto
-  then have "IO M1 s1 td \<inter> IO M1 s2 td = {}" using td_def by simp
-  moreover have "IO M2 t1 td \<subseteq> IO M1 s1 td" using red1 td_def by auto
-  moreover have "IO M2 t2 td \<subseteq> IO M1 s2 td" using red2 td_def by auto
-  ultimately have no_inter : "IO M2 t1 td \<inter> IO M2 t2 td = {}" by blast
+  obtain td where td_def : "td \<in> \<Omega> \<and> r_dist M1 td s1 s2" 
+    using rdist by auto
+  then have "IO M1 s1 td \<inter> IO M1 s2 td = {}" 
+    using td_def by simp
+  moreover have "IO M2 t1 td \<subseteq> IO M1 s1 td" 
+    using red1 td_def by auto
+  moreover have "IO M2 t2 td \<subseteq> IO M1 s2 td" 
+    using red2 td_def by auto
+  ultimately have no_inter : "IO M2 t1 td \<inter> IO M2 t2 td = {}" 
+    by blast
   
-  then have "td \<noteq> Leaf" by auto
-  then have "IO M2 t1 td \<noteq> {}" by (meson ap2 IO_applicable_nonempty applicable_set.elims(2) cs2 td_def assms(8)) 
-  then have "IO M2 t1 td \<noteq> IO M2 t2 td" using no_inter by auto 
-  then show ?thesis using no_inter td_def by auto 
+  then have "td \<noteq> Leaf" 
+    by auto
+  then have "IO M2 t1 td \<noteq> {}" 
+    by (meson ap2 IO_applicable_nonempty applicable_set.elims(2) cs2 td_def assms(8)) 
+  then have "IO M2 t1 td \<noteq> IO M2 t2 td" 
+    using no_inter by auto 
+  then show ?thesis 
+    using no_inter td_def by auto 
 qed
 
 
@@ -416,12 +474,14 @@ sequence to the first FSM are subsets of the analogously constructed response se
 FSM.
 \<close>
 
-fun atc_io_reduction_on :: "('in, 'out, 'state1) FSM \<Rightarrow> ('in, 'out, 'state2) FSM \<Rightarrow> 'in list \<Rightarrow> ('in, 'out) ATC set \<Rightarrow> bool" where
-"atc_io_reduction_on M1 M2 iseq \<Omega> = (LS\<^sub>i\<^sub>n M1 (initial M1) {iseq} \<subseteq> LS\<^sub>i\<^sub>n M2 (initial M2) {iseq} 
-  \<and> (\<forall> io \<in> LS\<^sub>i\<^sub>n M1 (initial M1) {iseq} . append_io_B M1 io \<Omega> \<subseteq> append_io_B M2 io \<Omega>))"
+fun atc_io_reduction_on :: "('in, 'out, 'state1) FSM \<Rightarrow> ('in, 'out, 'state2) FSM \<Rightarrow> 'in list 
+                            \<Rightarrow> ('in, 'out) ATC set \<Rightarrow> bool" where
+  "atc_io_reduction_on M1 M2 iseq \<Omega> = (LS\<^sub>i\<^sub>n M1 (initial M1) {iseq} \<subseteq> LS\<^sub>i\<^sub>n M2 (initial M2) {iseq} 
+    \<and> (\<forall> io \<in> LS\<^sub>i\<^sub>n M1 (initial M1) {iseq} . append_io_B M1 io \<Omega> \<subseteq> append_io_B M2 io \<Omega>))"
 
-fun atc_io_reduction_on_sets :: "('in, 'out, 'state1) FSM \<Rightarrow> 'in list set \<Rightarrow> ('in, 'out) ATC set \<Rightarrow> ('in, 'out, 'state2) FSM \<Rightarrow> bool" where
-"atc_io_reduction_on_sets M1 TS \<Omega> M2 = (\<forall> iseq \<in> TS . atc_io_reduction_on M1 M2 iseq \<Omega>)"
+fun atc_io_reduction_on_sets :: "('in, 'out, 'state1) FSM \<Rightarrow> 'in list set \<Rightarrow> ('in, 'out) ATC set 
+                                  \<Rightarrow> ('in, 'out, 'state2) FSM \<Rightarrow> bool" where
+  "atc_io_reduction_on_sets M1 TS \<Omega> M2 = (\<forall> iseq \<in> TS . atc_io_reduction_on M1 M2 iseq \<Omega>)"
 
 notation 
   atc_io_reduction_on_sets ("(_ \<preceq>\<lbrakk>_._\<rbrakk> _)" )
@@ -451,7 +511,9 @@ next
       using insert.IH by blast
   qed
   then have "LS\<^sub>i\<^sub>n M1 (initial M1) T \<subseteq> LS\<^sub>i\<^sub>n M2 (initial M2) (insert t T)"
-    by (meson insert_iff language_state_for_inputs_in_language_state language_state_for_inputs_map_fst language_state_for_inputs_map_fst_contained subsetCE subsetI) 
+    by (meson insert_iff language_state_for_inputs_in_language_state 
+        language_state_for_inputs_map_fst language_state_for_inputs_map_fst_contained 
+        subsetCE subsetI) 
   moreover have "LS\<^sub>i\<^sub>n M1 (initial M1) {t} \<subseteq> LS\<^sub>i\<^sub>n M2 (initial M2) (insert t T)"
   proof -
     obtain pps :: "('a \<times> 'b) list set \<Rightarrow> ('a \<times> 'b) list set \<Rightarrow> ('a \<times> 'b) list" where
@@ -461,13 +523,14 @@ next
       by blast
     moreover
     { assume "map fst (pps (L\<^sub>i\<^sub>n M2 (insert t T)) (L\<^sub>i\<^sub>n M1 {t})) \<notin> insert t T"
-      then have "pps (L\<^sub>i\<^sub>n M2 (insert t T)) (L\<^sub>i\<^sub>n M1 {t}) \<notin> L\<^sub>i\<^sub>n M1 {t} \<or> pps (L\<^sub>i\<^sub>n M2 (insert t T)) (L\<^sub>i\<^sub>n M1 {t}) \<in> L\<^sub>i\<^sub>n M2 (insert t T)"
+      then have "pps (L\<^sub>i\<^sub>n M2 (insert t T)) (L\<^sub>i\<^sub>n M1 {t}) \<notin> L\<^sub>i\<^sub>n M1 {t} 
+                      \<or> pps (L\<^sub>i\<^sub>n M2 (insert t T)) (L\<^sub>i\<^sub>n M1 {t}) \<in> L\<^sub>i\<^sub>n M2 (insert t T)"
         by (metis (no_types) insertI1 language_state_for_inputs_map_fst_contained singletonD) }
     ultimately show ?thesis
-      by (meson \<open>L\<^sub>i\<^sub>n M1 {t} \<subseteq> L\<^sub>i\<^sub>n M2 {t}\<close> language_state_for_inputs_in_language_state language_state_for_inputs_map_fst set_rev_mp)
+      by (meson \<open>L\<^sub>i\<^sub>n M1 {t} \<subseteq> L\<^sub>i\<^sub>n M2 {t}\<close> language_state_for_inputs_in_language_state 
+          language_state_for_inputs_map_fst set_rev_mp)
   qed
-    
-    
+        
      
   ultimately show ?case
   proof -
@@ -477,15 +540,29 @@ next
       "\<forall>x0 x1. (\<exists>v2. v2 \<in> x1 \<and> v2 \<notin> x0) = (pps x0 x1 \<in> x1 \<and> pps x0 x1 \<notin> x0)"
       by moura
     moreover
-    { assume "pps (LS\<^sub>i\<^sub>n M2 (initial M2) (insert t T)) (LS\<^sub>i\<^sub>n M1 (initial M1) (insert t T)) \<notin> LS\<^sub>i\<^sub>n M1 (initial M1) {t}"
+    { assume "pps (LS\<^sub>i\<^sub>n M2 (initial M2) (insert t T)) (LS\<^sub>i\<^sub>n M1 (initial M1) (insert t T)) 
+              \<notin> LS\<^sub>i\<^sub>n M1 (initial M1) {t}"
       moreover
-      { assume "map fst (pps (LS\<^sub>i\<^sub>n M2 (initial M2) (insert t T)) (LS\<^sub>i\<^sub>n M1 (initial M1) (insert t T))) \<notin> {t}"
-        then have "map fst (pps (LS\<^sub>i\<^sub>n M2 (initial M2) (insert t T)) (LS\<^sub>i\<^sub>n M1 (initial M1) (insert t T))) \<noteq> t"
+      { assume "map fst (pps (LS\<^sub>i\<^sub>n M2 (initial M2) (insert t T)) (LS\<^sub>i\<^sub>n M1 (initial M1) (insert t T))) 
+                \<notin> {t}"
+        then have "map fst (pps (LS\<^sub>i\<^sub>n M2 (initial M2) (insert t T)) 
+                      (LS\<^sub>i\<^sub>n M1 (initial M1) (insert t T))) \<noteq> t"
           by blast
-        then have "pps (LS\<^sub>i\<^sub>n M2 (initial M2) (insert t T)) (LS\<^sub>i\<^sub>n M1 (initial M1) (insert t T)) \<notin> LS\<^sub>i\<^sub>n M1 (initial M1) (insert t T) \<or> pps (LS\<^sub>i\<^sub>n M2 (initial M2) (insert t T)) (LS\<^sub>i\<^sub>n M1 (initial M1) (insert t T)) \<in> LS\<^sub>i\<^sub>n M2 (initial M2) (insert t T)"
-          using f1 by (meson \<open>LS\<^sub>i\<^sub>n M1 (initial M1) T \<subseteq> LS\<^sub>i\<^sub>n M2 (initial M2) (insert t T)\<close> insertE language_state_for_inputs_in_language_state language_state_for_inputs_map_fst language_state_for_inputs_map_fst_contained) }
-      ultimately have "io_reduction_on M1 (insert t T) M2 \<or> pps (LS\<^sub>i\<^sub>n M2 (initial M2) (insert t T)) (LS\<^sub>i\<^sub>n M1 (initial M1) (insert t T)) \<notin> LS\<^sub>i\<^sub>n M1 (initial M1) (insert t T) \<or> pps (LS\<^sub>i\<^sub>n M2 (initial M2) (insert t T)) (LS\<^sub>i\<^sub>n M1 (initial M1) (insert t T)) \<in> LS\<^sub>i\<^sub>n M2 (initial M2) (insert t T)"
-        using f1 by (meson language_state_for_inputs_in_language_state language_state_for_inputs_map_fst) }
+        then have "pps (LS\<^sub>i\<^sub>n M2 (initial M2) (insert t T)) (LS\<^sub>i\<^sub>n M1 (initial M1) (insert t T)) 
+                        \<notin> LS\<^sub>i\<^sub>n M1 (initial M1) (insert t T) 
+                    \<or> pps (LS\<^sub>i\<^sub>n M2 (initial M2) (insert t T)) (LS\<^sub>i\<^sub>n M1 (initial M1) (insert t T)) 
+                          \<in> LS\<^sub>i\<^sub>n M2 (initial M2) (insert t T)"
+          using f1 by (meson \<open>LS\<^sub>i\<^sub>n M1 (initial M1) T \<subseteq> LS\<^sub>i\<^sub>n M2 (initial M2) (insert t T)\<close> 
+                       insertE language_state_for_inputs_in_language_state 
+                       language_state_for_inputs_map_fst 
+                       language_state_for_inputs_map_fst_contained) }
+      ultimately have "io_reduction_on M1 (insert t T) M2 
+                        \<or> pps (LS\<^sub>i\<^sub>n M2 (initial M2) (insert t T)) (LS\<^sub>i\<^sub>n M1 (initial M1) (insert t T)) 
+                            \<notin> LS\<^sub>i\<^sub>n M1 (initial M1) (insert t T) 
+                        \<or> pps (LS\<^sub>i\<^sub>n M2 (initial M2) (insert t T)) (LS\<^sub>i\<^sub>n M1 (initial M1) (insert t T)) 
+                            \<in> LS\<^sub>i\<^sub>n M2 (initial M2) (insert t T)"
+        using f1 by (meson language_state_for_inputs_in_language_state 
+                     language_state_for_inputs_map_fst) }
       ultimately show ?thesis
         using f1 by (meson \<open>LS\<^sub>i\<^sub>n M1 (initial M1) {t} \<subseteq> LS\<^sub>i\<^sub>n M2 (initial M2) (insert t T)\<close> subsetI)
   qed 
@@ -508,50 +585,73 @@ lemma atc_reaction_reduction[intro] :
 shows "atc_reaction M2 q2 t io"
 using assms proof (induction t arbitrary: io q1 q2)
   case Leaf
-  then have "io = []" by (metis atc_reaction_nonempty_no_leaf list.exhaust) 
-  then show ?case by (simp add: leaf)  
+  then have "io = []" 
+    by (metis atc_reaction_nonempty_no_leaf list.exhaust) 
+  then show ?case 
+    by (simp add: leaf)  
 next
   case (Node x f)
-  then obtain io_hd io_tl where io_split : "io = io_hd # io_tl" by (metis ATC.distinct(1) atc_reaction_empty list.exhaust) 
-  moreover obtain y where y_def : "io_hd = (x,y)" using Node calculation by (metis ATC.inject atc_reaction_nonempty surj_pair) 
-  ultimately  obtain q1x where q1x_def : "q1x \<in> succ M1 (x,y) q1" "atc_reaction M1 q1x (f y) io_tl" using Node.prems(4) by blast 
+  then obtain io_hd io_tl where io_split : "io = io_hd # io_tl" 
+    by (metis ATC.distinct(1) atc_reaction_empty list.exhaust) 
+  moreover obtain y where y_def : "io_hd = (x,y)" 
+    using Node calculation by (metis ATC.inject atc_reaction_nonempty surj_pair) 
+  ultimately  obtain q1x where q1x_def : "q1x \<in> succ M1 (x,y) q1" "atc_reaction M1 q1x (f y) io_tl" 
+    using Node.prems(4) by blast 
 
-  then have pt1 : "path M1 ([(x,y)] || [q1x]) q1" by auto
-  then have ls1 : "[(x,y)] \<in> language_state M1 q1" unfolding language_state_def path_def using list.simps(9) by force
-  moreover have "q1x \<in> io_targets M1 q1 [(x,y)]" unfolding io_targets.simps
+  then have pt1 : "path M1 ([(x,y)] || [q1x]) q1" 
+    by auto
+  then have ls1 : "[(x,y)] \<in> language_state M1 q1" 
+    unfolding language_state_def path_def using list.simps(9) by force
+  moreover have "q1x \<in> io_targets M1 q1 [(x,y)]" 
+    unfolding io_targets.simps
   proof -
     have f1: "length [(x, y)] = length [q1x]"
       by simp
     have "q1x = target ([(x, y)] || [q1x]) q1"
       by simp
-    then show "q1x \<in> {target ([(x, y)] || cs) q1 |cs. path M1 ([(x, y)] || cs) q1 \<and> length [(x, y)] = length cs}"
+    then show "q1x \<in> {target ([(x, y)] || cs) q1 |cs. path M1 ([(x, y)] || cs) q1 
+                                                      \<and> length [(x, y)] = length cs}"
       using f1 pt1 by blast
   qed 
-  ultimately have tgt1 : "io_targets M1 q1 [(x,y)] = {q1x}" using Node.prems io_targets_observable_singleton_ex q1x_def 
+  ultimately have tgt1 : "io_targets M1 q1 [(x,y)] = {q1x}" 
+    using Node.prems io_targets_observable_singleton_ex q1x_def 
     by (metis (no_types, lifting) singletonD) 
 
   
-  then have ls2 : "[(x,y)] \<in> language_state M2 q2" using Node.prems(1) ls1 by auto
-  then obtain q2x where q2x_def : "q2x \<in> succ M2 (x,y) q2" unfolding language_state_def path_def using transition_system.path.cases by fastforce 
-  then have pt2 : "path M2 ([(x,y)] || [q2x]) q2" by auto
-  then have "q2x \<in> io_targets M2 q2 [(x,y)]" using ls2 unfolding io_targets.simps 
+  then have ls2 : "[(x,y)] \<in> language_state M2 q2" 
+    using Node.prems(1) ls1 by auto
+  then obtain q2x where q2x_def : "q2x \<in> succ M2 (x,y) q2" 
+    unfolding language_state_def path_def 
+    using transition_system.path.cases by fastforce 
+  then have pt2 : "path M2 ([(x,y)] || [q2x]) q2" 
+    by auto
+  then have "q2x \<in> io_targets M2 q2 [(x,y)]" 
+    using ls2 unfolding io_targets.simps 
   proof -
     have f1: "length [(x, y)] = length [q2x]"
       by simp
     have "q2x = target ([(x, y)] || [q2x]) q2"
       by simp
-    then show "q2x \<in> {target ([(x, y)] || cs) q2 |cs. path M2 ([(x, y)] || cs) q2 \<and> length [(x, y)] = length cs}"
+    then show "q2x \<in> {target ([(x, y)] || cs) q2 |cs. path M2 ([(x, y)] || cs) q2 
+                                                        \<and> length [(x, y)] = length cs}"
       using f1 pt2 by blast
   qed
 
-  then have tgt2 : "io_targets M2 q2 [(x,y)] = {q2x}" using Node.prems io_targets_observable_singleton_ex ls2 q2x_def 
+  then have tgt2 : "io_targets M2 q2 [(x,y)] = {q2x}" 
+    using Node.prems io_targets_observable_singleton_ex ls2 q2x_def 
     by (metis (no_types, lifting) singletonD) 
 
 
-  then have "language_state M1 q1x \<subseteq> language_state M2 q2x" using language_state_inclusion_of_state_reached_by_same_sequence[of M1 q1 M2 q2 "[(x,y)]" q1x q2x] tgt1 tgt2 Node.prems by auto
-  moreover have "q1x \<in> nodes M1" using q1x_def(1) Node.prems(2) by (metis insertI1 io_targets_nodes tgt1)
-  moreover have "q2x \<in> nodes M2" using q2x_def(1) Node.prems(3) by (metis insertI1 io_targets_nodes tgt2)
-  ultimately have "q2x \<in> succ M2 (x,y) q2 \<and> atc_reaction M2 q2x (f y) io_tl" using Node.IH[of "f y" q1x q2x io_tl] ob1 ob2 q1x_def(2) q2x_def by blast 
+  then have "language_state M1 q1x \<subseteq> language_state M2 q2x" 
+    using language_state_inclusion_of_state_reached_by_same_sequence
+          [of M1 q1 M2 q2 "[(x,y)]" q1x q2x] 
+          tgt1 tgt2 Node.prems by auto
+  moreover have "q1x \<in> nodes M1" 
+    using q1x_def(1) Node.prems(2) by (metis insertI1 io_targets_nodes tgt1)
+  moreover have "q2x \<in> nodes M2" 
+    using q2x_def(1) Node.prems(3) by (metis insertI1 io_targets_nodes tgt2)
+  ultimately have "q2x \<in> succ M2 (x,y) q2 \<and> atc_reaction M2 q2x (f y) io_tl" 
+    using Node.IH[of "f y" q1x q2x io_tl] ob1 ob2 q1x_def(2) q2x_def by blast 
  
 
   then show "atc_reaction M2 q2 (Node x f) io" using io_split y_def by blast 
@@ -575,8 +675,10 @@ lemma IO_set_reduction :
   and     ob2 : "observable M2"
 shows "IO_set M1 q1 \<Omega> \<subseteq> IO_set M2 q2 \<Omega>"
 proof -
-  have "\<forall> t \<in> \<Omega> . IO M1 q1 t \<subseteq> IO M2 q2 t" using assms IO_reduction by metis 
-  then show ?thesis unfolding IO_set.simps by blast
+  have "\<forall> t \<in> \<Omega> . IO M1 q1 t \<subseteq> IO M2 q2 t" 
+    using assms IO_reduction by metis 
+  then show ?thesis 
+    unfolding IO_set.simps by blast
 qed
 
 lemma B_reduction :
@@ -586,27 +688,42 @@ lemma B_reduction :
 shows "B M1 io \<Omega> \<subseteq> B M2 io \<Omega>"
 proof 
   fix xy assume xy_assm : "xy \<in> B M1 io \<Omega>"
-  then obtain q1x where q1x_def : "q1x \<in> (io_targets M1 (initial M1) io) \<and> xy \<in> IO_set M1 q1x \<Omega>" unfolding B.simps by auto
-  then obtain tr1 where tr1_def : "path M1 (io || tr1) (initial M1) \<and> length io = length tr1" by auto
+  then obtain q1x where q1x_def : "q1x \<in> (io_targets M1 (initial M1) io) \<and> xy \<in> IO_set M1 q1x \<Omega>" 
+    unfolding B.simps by auto
+  then obtain tr1 where tr1_def : "path M1 (io || tr1) (initial M1) \<and> length io = length tr1" 
+    by auto
 
-  then have q1x_ob : "io_targets M1 (initial M1) io = {q1x}" using assms
+  then have q1x_ob : "io_targets M1 (initial M1) io = {q1x}" 
+    using assms
     by (metis io_targets_observable_singleton_ex language_state q1x_def singleton_iff) 
   
-  then have ls1 : "io \<in> language_state M1 (initial M1)" by auto 
-  then have ls2 : "io \<in> language_state M2 (initial M2)" using red by auto
+  then have ls1 : "io \<in> language_state M1 (initial M1)" 
+    by auto 
+  then have ls2 : "io \<in> language_state M2 (initial M2)" 
+    using red by auto
 
-  then obtain tr2 where tr2_def : "path M2 (io || tr2) (initial M2) \<and> length io = length tr2" by auto
-  then obtain q2x where q2x_def : "q2x \<in> (io_targets M2 (initial M2) io)" by auto
+  then obtain tr2 where tr2_def : "path M2 (io || tr2) (initial M2) \<and> length io = length tr2" 
+    by auto
+  then obtain q2x where q2x_def : "q2x \<in> (io_targets M2 (initial M2) io)" 
+    by auto
 
-  then have q2x_ob : "io_targets M2 (initial M2) io = {q2x}" using tr2_def assms
+  then have q2x_ob : "io_targets M2 (initial M2) io = {q2x}" 
+    using tr2_def assms
     by (metis io_targets_observable_singleton_ex language_state singleton_iff) 
 
-  then have "language_state M1 q1x \<subseteq> language_state M2 q2x" using q1x_ob assms unfolding io_reduction.simps by (simp add: language_state_inclusion_of_state_reached_by_same_sequence) 
-  then have "IO_set M1 q1x \<Omega> \<subseteq> IO_set M2 q2x \<Omega>" using assms IO_set_reduction by (metis FSM.nodes.initial io_targets_nodes q1x_def q2x_def) 
-  moreover have "B M1 io \<Omega> = IO_set M1 q1x \<Omega>" using q1x_ob by auto
-  moreover have "B M2 io \<Omega> = IO_set M2 q2x \<Omega>" using q2x_ob by auto
-  ultimately have "B M1 io \<Omega> \<subseteq> B M2 io \<Omega>" by simp
-  then show "xy \<in> B M2 io \<Omega>" using xy_assm by blast
+  then have "language_state M1 q1x \<subseteq> language_state M2 q2x" 
+    using q1x_ob assms unfolding io_reduction.simps 
+    by (simp add: language_state_inclusion_of_state_reached_by_same_sequence) 
+  then have "IO_set M1 q1x \<Omega> \<subseteq> IO_set M2 q2x \<Omega>" 
+    using assms IO_set_reduction by (metis FSM.nodes.initial io_targets_nodes q1x_def q2x_def) 
+  moreover have "B M1 io \<Omega> = IO_set M1 q1x \<Omega>" 
+    using q1x_ob by auto
+  moreover have "B M2 io \<Omega> = IO_set M2 q2x \<Omega>" 
+    using q2x_ob by auto
+  ultimately have "B M1 io \<Omega> \<subseteq> B M2 io \<Omega>" 
+    by simp
+  then show "xy \<in> B M2 io \<Omega>" using xy_assm 
+    by blast
 qed
 
 
@@ -617,9 +734,12 @@ lemma append_io_B_reduction :
 shows "append_io_B M1 io \<Omega> \<subseteq> append_io_B M2 io \<Omega>"
 proof 
   fix ioR assume ioR_assm : "ioR \<in> append_io_B M1 io \<Omega>" 
-  then obtain res where res_def : "ioR = io @ res" "res \<in> B M1 io \<Omega>" by auto
-  then have "res \<in> B M2 io \<Omega>" using assms B_reduction by (metis (no_types, hide_lams) subset_iff)
-  then show "ioR \<in> append_io_B M2 io \<Omega>" using ioR_assm res_def by auto
+  then obtain res where res_def : "ioR = io @ res" "res \<in> B M1 io \<Omega>" 
+    by auto
+  then have "res \<in> B M2 io \<Omega>" 
+    using assms B_reduction by (metis (no_types, hide_lams) subset_iff)
+  then show "ioR \<in> append_io_B M2 io \<Omega>" 
+    using ioR_assm res_def by auto
 qed 
 
 
@@ -630,9 +750,11 @@ lemma atc_io_reduction_on_reduction[intro] :
   and     ob2 : "observable M2"
 shows "atc_io_reduction_on M1 M2 iseq \<Omega>"
 unfolding atc_io_reduction_on.simps proof 
-  show "LS\<^sub>i\<^sub>n M1 (initial M1) {iseq} \<subseteq> LS\<^sub>i\<^sub>n M2 (initial M2) {iseq}" using red by auto 
+  show "LS\<^sub>i\<^sub>n M1 (initial M1) {iseq} \<subseteq> LS\<^sub>i\<^sub>n M2 (initial M2) {iseq}" 
+    using red by auto 
 next
-  show "\<forall>io\<in>LS\<^sub>i\<^sub>n M1 (initial M1) {iseq}. append_io_B M1 io \<Omega> \<subseteq> append_io_B M2 io \<Omega>" using  append_io_B_reduction assms by blast
+  show "\<forall>io\<in>LS\<^sub>i\<^sub>n M1 (initial M1) {iseq}. append_io_B M1 io \<Omega> \<subseteq> append_io_B M2 io \<Omega>" 
+    using  append_io_B_reduction assms by blast
 qed
     
 
@@ -645,16 +767,22 @@ shows "atc_io_reduction_on_sets M1 TS \<Omega> M2"
 
 lemma atc_io_reduction_on_sets_via_LS\<^sub>i\<^sub>n : 
   assumes "atc_io_reduction_on_sets M1 TS \<Omega> M2"
-  shows "(L\<^sub>i\<^sub>n M1 TS \<union> (\<Union>io\<in>LS\<^sub>i\<^sub>n M1 (initial M1) TS. append_io_B M1 io \<Omega>)) \<subseteq> (L\<^sub>i\<^sub>n M2 TS \<union> (\<Union>io\<in>LS\<^sub>i\<^sub>n M2 (initial M2) TS. append_io_B M2 io \<Omega>))"
+  shows "(L\<^sub>i\<^sub>n M1 TS \<union> (\<Union>io\<in>LS\<^sub>i\<^sub>n M1 (initial M1) TS. append_io_B M1 io \<Omega>)) 
+          \<subseteq> (L\<^sub>i\<^sub>n M2 TS \<union> (\<Union>io\<in>LS\<^sub>i\<^sub>n M2 (initial M2) TS. append_io_B M2 io \<Omega>))"
 proof -
   have "\<forall> iseq \<in> TS . (LS\<^sub>i\<^sub>n M1 (initial M1) {iseq} \<subseteq> LS\<^sub>i\<^sub>n M2 (initial M2) {iseq} 
-                        \<and> (\<forall> io \<in> LS\<^sub>i\<^sub>n M1 (initial M1) {iseq} . append_io_B M1 io \<Omega> \<subseteq> append_io_B M2 io \<Omega>))" 
+                        \<and> (\<forall> io \<in> LS\<^sub>i\<^sub>n M1 (initial M1) {iseq} . append_io_B M1 io \<Omega> 
+                            \<subseteq> append_io_B M2 io \<Omega>))" 
     using assms by auto
-  then have "\<forall> iseq \<in> TS . (\<Union>io\<in>LS\<^sub>i\<^sub>n M1 (initial M1) {iseq}. append_io_B M1 io \<Omega>) \<subseteq> (\<Union>io\<in>LS\<^sub>i\<^sub>n M2 (initial M2) {iseq}. append_io_B M2 io \<Omega>)"
+  then have "\<forall> iseq \<in> TS . (\<Union>io\<in>LS\<^sub>i\<^sub>n M1 (initial M1) {iseq}. append_io_B M1 io \<Omega>) 
+                            \<subseteq> (\<Union>io\<in>LS\<^sub>i\<^sub>n M2 (initial M2) {iseq}. append_io_B M2 io \<Omega>)"
     by blast
-  moreover have "\<forall> iseq \<in> TS . (\<Union>io\<in>LS\<^sub>i\<^sub>n M2 (initial M2) {iseq}. append_io_B M2 io \<Omega>) \<subseteq> (\<Union>io\<in>LS\<^sub>i\<^sub>n M2 (initial M2) TS. append_io_B M2 io \<Omega>)"
+  moreover have "\<forall> iseq \<in> TS . (\<Union>io\<in>LS\<^sub>i\<^sub>n M2 (initial M2) {iseq}. append_io_B M2 io \<Omega>) 
+                                \<subseteq> (\<Union>io\<in>LS\<^sub>i\<^sub>n M2 (initial M2) TS. append_io_B M2 io \<Omega>)"
     unfolding language_state_for_inputs.simps by blast
-  ultimately have elem_subset : "\<forall> iseq \<in> TS . (\<Union>io\<in>LS\<^sub>i\<^sub>n M1 (initial M1) {iseq}. append_io_B M1 io \<Omega>) \<subseteq> (\<Union>io\<in>LS\<^sub>i\<^sub>n M2 (initial M2) TS. append_io_B M2 io \<Omega>)" 
+  ultimately have elem_subset : "\<forall> iseq \<in> TS . 
+                                  (\<Union>io\<in>LS\<^sub>i\<^sub>n M1 (initial M1) {iseq}. append_io_B M1 io \<Omega>) 
+                                    \<subseteq> (\<Union>io\<in>LS\<^sub>i\<^sub>n M2 (initial M2) TS. append_io_B M2 io \<Omega>)" 
     by blast
   
   show ?thesis
@@ -670,7 +798,11 @@ proof -
       then have "L\<^sub>i\<^sub>n M1 {iseq} \<subseteq> L\<^sub>i\<^sub>n M2 {iseq}" 
         by auto
       then have "x \<in> L\<^sub>i\<^sub>n M2 TS"
-        by (metis (no_types, lifting) UN_I \<open>\<And>thesis. (\<And>iseq. \<lbrakk>iseq \<in> TS; x \<in> L\<^sub>i\<^sub>n M1 {iseq}\<rbrakk> \<Longrightarrow> thesis) \<Longrightarrow> thesis\<close> \<open>\<forall>iseq\<in>TS. L\<^sub>i\<^sub>n M1 {iseq} \<subseteq> L\<^sub>i\<^sub>n M2 {iseq} \<and> (\<forall>io\<in>L\<^sub>i\<^sub>n M1 {iseq}. append_io_B M1 io \<Omega> \<subseteq> append_io_B M2 io \<Omega>)\<close> language_state_for_input_alt_def language_state_for_inputs_alt_def set_rev_mp) 
+        by (metis (no_types, lifting) UN_I 
+            \<open>\<And>thesis. (\<And>iseq. \<lbrakk>iseq \<in> TS; x \<in> L\<^sub>i\<^sub>n M1 {iseq}\<rbrakk> \<Longrightarrow> thesis) \<Longrightarrow> thesis\<close> 
+            \<open>\<forall>iseq\<in>TS. L\<^sub>i\<^sub>n M1 {iseq} \<subseteq> L\<^sub>i\<^sub>n M2 {iseq} \<and> (\<forall>io\<in>L\<^sub>i\<^sub>n M1 {iseq}. append_io_B M1 io \<Omega> 
+                                                                            \<subseteq> append_io_B M2 io \<Omega>)\<close> 
+            language_state_for_input_alt_def language_state_for_inputs_alt_def set_rev_mp) 
       then show ?thesis 
         by blast
     next
